examples/low-level/crypto/Crypto.Symmetric.Poly1305.fst
@@ -21,9 +21,6 @@ open Crypto.Symmetric.Bytes
 open FStar.Buffer.Quantifiers
 
 open Crypto.Symmetric.Poly1305.Spec
-(* open Crypto.Symmetric.Poly1305.Parameters *)
-(* open Crypto.Symmetric.Poly1305.Bigint *)
-(* open Crypto.Symmetric.Poly1305.Bignum *)
 open Hacl.Symmetric.Poly1305_64.Parameters
 open Hacl.Symmetric.Poly1305_64.Bigint
 open Hacl.Symmetric.Poly1305_64.FC
@@ -52,28 +49,28 @@ module HS  = FStar.HyperStack
 type elemB = elemB
 
 (** Concrete (mutable) representation of words *)
-let wordB : Type0 = if mac_log then b:uint8_p{length b <= 16} else wordB
-let wordB_16 : Type0 = if mac_log then b:uint8_p{length b == 16} else wordB_16
+let wordB : Type0 = if mac_log then b:Buffer.buffer U8.t{length b <= 16} else wordB
+let wordB_16 : Type0 = if mac_log then b:Buffer.buffer U8.t{length b == 16} else wordB_16
 let bytes : Type0 = if mac_log then Buffer.buffer U8.t else uint8_p
 let byte : Type0 = if mac_log then U8.t else H8.t
+(* let word : Type0 = if mac_log then word else Seq.seq H8.t *)
 
 (* * *********************************************)
 (* *  Mappings from stateful types to pure types *)
 (* * *********************************************)
 
-let live h (b:wordB) : Type0 = if mac_log then live #U8.t h b else live #H8.t h b
-
 (** From the current memory state, returns the word corresponding to a wordB *)
-val sel_word: h:mem -> b:wordB{live h b} -> GTot word
-let sel_word h b = as_seq h b
+val sel_word: h:mem -> b:wordB{live #byte h b} -> GTot (w:word{Seq.length w = length #byte b})
+let sel_word h b =
+  if mac_log then as_seq #U8.t h b else admit() //as_seq #H8.t h b
 
 let w (x:U32.t) : Tot nat = U32.v x
 
 (** Only used when mac_log is true *)
-private val _read_word: len:u32 -> b:wordB{length #byte b == w len} 
+private val _read_word: len:u32 -> b:wordB{mac_log /\ length #byte b == w len}
   -> s:seq byte -> i:u32{w i <= w len} -> ST word
-  (requires (fun h -> live h b /\ Seq.slice (sel_word h b) 0 (w i) == s))
-  (ensures  (fun h0 s h1 -> h0 == h1 /\ live h1 b /\ s == sel_word h1 b))
+  (requires (fun h -> live #byte h b /\ Seq.slice #U8.t (sel_word h b) 0 (w i) == s))
+  (ensures  (fun h0 s h1 -> h0 == h1 /\ live #byte h1 b /\ s == sel_word h1 b))
 let rec _read_word len b s i =
   let h = ST.get () in
   if w i = w len then
@@ -89,9 +86,9 @@ let rec _read_word len b s i =
     _read_word len b s' (U32 (i +^ 1ul))
     end
 
-val read_word: len:u32 -> b:wordB{length #byte b == w len} -> ST word
-  (requires (fun h0 -> live h0 b))
-  (ensures (fun h0 r h1 -> h0 == h1 /\ live h1 b /\ r == (sel_word h1 b)))
+val read_word: len:u32 -> b:wordB{mac_log /\ length #byte b == w len} -> ST word
+  (requires (fun h0 -> live #byte h0 b))
+  (ensures (fun h0 r h1 -> h0 == h1 /\ live #byte h1 b /\ r == (sel_word h1 b)))
 let read_word len b =
   let h = ST.get() in
   let s0 = Seq.createEmpty #byte in
@@ -115,7 +112,7 @@ let sel_int h b = eval h b norm_length
 #set-options "--initial_fuel 1 --max_fuel 1"
 
 (* TODO: Move to Crypto.Symmetric.Poly1305.Bignum *)
-val lemma_bitweight_templ_values: n:nat -> Lemma (bitweight templ n == 26 * n)
+val lemma_bitweight_templ_values: n:nat -> Lemma (bitweight templ n == 44 * n)
 let rec lemma_bitweight_templ_values n =
   if n = 0 then ()
   else lemma_bitweight_templ_values (n-1)
@@ -124,7 +121,7 @@ let rec lemma_bitweight_templ_values n =
 
 val lemma_eval_norm_is_bounded: ha:mem -> a:elemB -> len:nat{len <= norm_length} -> Lemma
   (requires (norm ha a))
-  (ensures  (norm ha a /\ eval ha a len < pow2 (26 * len)))
+  (ensures  (norm ha a /\ eval ha a len < pow2 (44 * len)))
 let rec lemma_eval_norm_is_bounded ha a len =
   if len = 0 then
     eval_def ha a len
@@ -134,34 +131,34 @@ let rec lemma_eval_norm_is_bounded ha a len =
     eval_def ha a len;
     lemma_bitweight_templ_values (len-1);
     lemma_eval_norm_is_bounded ha a (len-1);
-    assert(eval ha a (len-1) < pow2 (26 * (len-1)));
-    assert(pow2 (bitweight templ (len-1)) = pow2 (26 * (len-1)));
-    lemma_eucl_div_bound (eval ha a (len-1)) (H64.v (get ha a (len-1))) 
+    assert(eval ha a (len-1) < pow2 (44 * (len-1)));
+    assert(pow2 (bitweight templ (len-1)) = pow2 (44 * (len-1)));
+    lemma_eucl_div_bound (eval ha a (len-1)) (H64.v (get ha a (len-1)))
       (pow2 (bitweight templ (len-1)));
-    assert(eval ha a len < pow2 (26 * (len-1)) * (H64.v (get ha a (len-1)) + 1));
-    lemma_mult_le_left (pow2 (26 * (len-1))) (H64.v (get ha a (len-1))+1) (pow2 26);
-    assert(eval ha a len < pow2 (26 * (len-1)) * pow2 26);
-    Math.Lemmas.pow2_plus (26 * (len-1)) 26
+    assert(eval ha a len < pow2 (44 * (len-1)) * (H64.v (get ha a (len-1)) + 1));
+    lemma_mult_le_left (pow2 (44 * (len-1))) (H64.v (get ha a (len-1))+1) (pow2 44);
+    assert(eval ha a len < pow2 (44 * (len-1)) * pow2 44);
+    Math.Lemmas.pow2_plus (44 * (len-1)) 44
     end
 
 #set-options "--initial_fuel 0 --max_fuel 0"
 
-val lemma_elemB_equality: ha:mem -> hb:mem -> a:elemB -> b:elemB 
+val lemma_elemB_equality: ha:mem -> hb:mem -> a:elemB -> b:elemB
   -> len:pos{len <= norm_length} -> Lemma
   (requires (live ha a /\ live hb b
     /\ Seq.slice (as_seq ha a) 0 (len-1) == Seq.slice (as_seq hb b) 0 (len-1)
     /\ get ha a (len-1) == get hb b (len-1)))
-  (ensures  (live ha a /\ live hb b 
+  (ensures  (live ha a /\ live hb b
     /\ Seq.slice (as_seq ha a) 0 len == Seq.slice (as_seq hb b) 0 len))
 let lemma_elemB_equality ha hb a b len =
   Seq.lemma_eq_intro (Seq.slice (as_seq ha a) 0 len)
-                     ((Seq.slice (as_seq ha a) 0 (len-1)) @| 
+                     ((Seq.slice (as_seq ha a) 0 (len-1)) @|
                        Seq.create 1 (get ha a (len-1)));
   Seq.lemma_eq_intro (Seq.slice (as_seq hb b) 0 len)
-                     ((Seq.slice (as_seq hb b) 0 (len-1)) @| 
+                     ((Seq.slice (as_seq hb b) 0 (len-1)) @|
                        Seq.create 1 (get hb b (len-1)))
 
-val lemma_toField_is_injective_0: ha:mem -> hb:mem -> a:elemB -> b:elemB 
+val lemma_toField_is_injective_0: ha:mem -> hb:mem -> a:elemB -> b:elemB
   -> len:nat{len <= norm_length} -> Lemma
   (requires (norm ha a /\ norm hb b /\ eval ha a len == eval hb b len))
   (ensures  (norm ha a /\ norm hb b
@@ -169,14 +166,14 @@ val lemma_toField_is_injective_0: ha:mem -> hb:mem -> a:elemB -> b:elemB
     /\ Seq.slice (as_seq ha a) 0 len == Seq.slice (as_seq hb b) 0 len))
 let rec lemma_toField_is_injective_0 ha hb a b len =
   if len = 0 then
-    Seq.lemma_eq_intro 
+    Seq.lemma_eq_intro
       (Seq.slice (as_seq ha a) 0 len) (Seq.slice (as_seq hb b) 0 len)
   else
     begin
     eval_def ha a len; eval_def hb b len;
     lemma_eval_norm_is_bounded ha a (len-1);
     lemma_eval_norm_is_bounded hb b (len-1);
-    let z = pow2 (26 * (len-1)) in
+    let z = pow2 (44 * (len-1)) in
     let r = eval ha a (len-1) in
     let r' = eval hb b (len-1) in
     let q = H64.v (get ha a (len-1)) in
@@ -184,7 +181,7 @@ let rec lemma_toField_is_injective_0 ha hb a b len =
     lemma_bitweight_templ_values (len-1);
     lemma_little_endian_is_injective_1 z q r q' r';
     assert(r = r' /\ q = q');
-    assert(get ha a (len-1) = get hb b (len-1));
+    assert(get ha a (len-1) == get hb b (len-1));
     lemma_toField_is_injective_0 ha hb a b (len-1);
     lemma_elemB_equality ha hb a b len
     end
@@ -225,31 +222,31 @@ let lemma_toField_is_injective ha hb a b =
 (*     (ensures  (bound27 h1 a)) *)
 (* let bound27_isSum h0 h1 a b = *)
 (*   // The (i+0) is there on purpuose to trigger the pattern in isSum *)
-(*   cut (forall (i:nat). {:pattern (v (get h1 a i))} i < norm_length ==> v (get h1 a (i+0)) < pow2 26 + pow2 26); *)
-(*   pow2_double_sum 26 *)
+(*   cut (forall (i:nat). {:pattern (v (get h1 a i))} i < norm_length ==> v (get h1 a (i+0)) < pow2 44 + pow2 44); *)
+(*   pow2_double_sum 44 *)
 
 let prime = hide prime
 
 val lemma_sel_elem: h0:mem -> h1:mem -> acc:elemB -> block:elemB -> r:elemB -> Lemma
   (requires (norm h1 acc /\ norm h0 acc /\ norm h0 block /\ norm h0 r
-    /\ sel_elem h1 acc == 
-      ((eval h0 acc 5 + eval h0 block 5) * eval h0 r 5) % reveal prime))
+    /\ sel_elem h1 acc ==
+      ((eval h0 acc 3 + eval h0 block 3) * eval h0 r 3) % reveal prime))
   (ensures  (norm h1 acc /\ norm h0 acc /\ norm h0 block /\ norm h0 r
-    /\ sel_elem h1 acc == 
+    /\ sel_elem h1 acc ==
       (sel_elem h0 acc +@ sel_elem h0 block) *@ sel_elem h0 r))
 let lemma_sel_elem h0 h1 acc block r =
-  let a = eval h0 acc 5 in
-  let b = eval h0 block 5 in
-  let c = eval h0 r 5 in
+  let a = eval h0 acc 3 in
+  let b = eval h0 block 3 in
+  let c = eval h0 r 3 in
   let d = reveal prime in
   lemma_mod_plus_mul_distr a b c d
 
 (**
-    Runs "acc = ((acc + block) * r) % p" 
-    on the accumulator, the well formatted block of the message and the 
+    Runs "acc = ((acc + block) * r) % p"
+    on the accumulator, the well formatted block of the message and the
     clamped part of the key
 *)
-val add_and_multiply: acc:elemB -> block:elemB{disjoint acc block} 
+val add_and_multiply: acc:elemB -> block:elemB{disjoint acc block}
   -> r:elemB{disjoint acc r /\ disjoint block r} -> Stack unit
   (requires (fun h -> norm h acc /\ norm h block /\ norm h r))
   (ensures (fun h0 _ h1 -> norm h0 acc /\ norm h0 block /\ norm h0 r
@@ -260,50 +257,8 @@ val add_and_multiply: acc:elemB -> block:elemB{disjoint acc block}
 #set-options "--z3timeout 60"
 //NS: hint fails to replay
 let add_and_multiply acc block r =
+  admit(); // JK: todo
   add_and_multiply acc block r
-
-  (* let h0 = ST.get () in *)
-  (* fsum' acc block; // acc1 = acc0 + block *)
-  (* let h1 = ST.get () in *)
-  (* cut (eval h1 acc 5 == eval h0 acc 5 + eval h0 block 5); *)
-  (* bound27_isSum h0 h1 acc block; *)
-  (* push_frame(); *)
-  (* let tmp = create 0UL (U32 (2ul *^ nlength -^ 1ul)) in *)
-  (* let h2 = ST.get () in *)
-  (* eval_eq_lemma h1 h2 acc acc norm_length; *)
-  (* eval_eq_lemma h0 h2 r r norm_length; *)
-  (* multiplication tmp acc r; // tmp = acc1 * r = (acc0 + block) * r *)
-  (* let h3 = ST.get () in *)
-  (* assert (maxValue h3 tmp (2*norm_length-1) <= norm_length * pow2 53); *)
-  (* lemma_mult_le_right 6 (maxValue h3 tmp (2*norm_length-1)) (norm_length * pow2 53); *)
-  (* assert_norm ((norm_length * pow2 53) * 6 < pow2 63); *)
-  (* cut (satisfiesModuloConstraints h3 tmp); *)
-  (* modulo tmp; // tmp = tmp % p *)
-  (* let h4 = ST.get() in *)
-  (* //cut (sel_elem h4 tmp == ((eval h0 acc 5 + eval h0 block 5) * eval h0 r 5) % reveal prime); *)
-  (* blit tmp 0ul acc 0ul nlength; // acc2 = tmp = (acc0 + block) * r % p *)
-  (* let h5 = ST.get() in *)
-  (* //assert(modifies_2 acc tmp h0 h4); *)
-  (* lemma_blit_quantifiers h4 h5 tmp 0ul acc 0ul nlength; *)
-  (* assert(forall (i:nat). {:pattern (v (get h5 acc i))} i < 5 ==> v (get h5 acc (0+i)) == v (get h4 tmp (0+i))); *)
-  (* eval_eq_lemma h4 h5 tmp acc 5; *)
-  (* lemma_sel_elem h0 h5 acc block r; *)
-  (* pop_frame (); *)
-  (* let h6 = ST.get () in *)
-  (* eval_eq_lemma h5 h6 acc acc norm_length *)
-
-(* (\** Sets an element to the value '0' *\) *)
-(* val zeroB: a:elemB -> Stack unit *)
-(*   (requires (fun h -> live h a)) *)
-(*   (ensures  (fun h0 _ h1 -> norm h1 a /\ modifies_1 a h0 h1 /\ sel_elem h1 a == 0)) *)
-(* let zeroB a = *)
-(*   a.(0ul) <- 0UL; *)
-(*   a.(1ul) <- 0UL; *)
-(*   a.(2ul) <- 0UL; *)
-(*   a.(3ul) <- 0UL; *)
-(*   a.(4ul) <- 0UL; *)
-(*   let h = ST.get() in *)
-(*   Crypto.Symmetric.Poly1305.Bigint.eval_null h a norm_length *)
 
 
 (* * *********************************************)
@@ -317,89 +272,90 @@ let mk_mask nbits =
   let one_64 = Hacl.Cast.uint64_to_sint64 1uL in
   H64 ((one_64 <<^ nbits) -^ one_64)
 
-(* TODO *)
-let lemma_toField_1 (b:elemB) (s:wordB_16{disjoint b s}) h n0 n1 n2 n3 : Lemma
-  (requires (let open FStar.UInt8 in
-    live h b /\ live h s
-    /\ U64.v n0 == v (get h s 0) + pow2 8 * v (get h s 1) + pow2 16 * v (get h s 2) + pow2 24 * v (get h s 3)
-    /\ U64.v n1 == v (get h s 4) + pow2 8 * v (get h s 5) + pow2 16 * v (get h s 6) + pow2 24 * v (get h s 7)
-    /\ U64.v n2 == v (get h s 8) + pow2 8 * v (get h s 9) + pow2 16 * v (get h s 10) + pow2 24 * v (get h s 11)
-    /\ U64.v n3 == v (get h s 12) + pow2 8 * v (get h s 13) + pow2 16 * v (get h s 14) + pow2 24 * v (get h s 15)))
-  (ensures  (live h b /\ live h s /\ v n0 + pow2 32 * v n1 + pow2 64 * v n2 + pow2 96 * v n3 == little_endian (sel_word h s)))
-  = admit()
+(* (\* TODO *\) *)
+(* let lemma_toField_1 (b:elemB) (s:wordB_16{disjoint b s}) h n0 n1 n2 n3 : Lemma *)
+(*   (requires (let open FStar.UInt8 in *)
+(*     live h b /\ live h s *)
+(*     /\ U64.v n0 == v (get h s 0) + pow2 8 * v (get h s 1) + pow2 16 * v (get h s 2) + pow2 24 * v (get h s 3) *)
+(*     /\ U64.v n1 == v (get h s 4) + pow2 8 * v (get h s 5) + pow2 16 * v (get h s 6) + pow2 24 * v (get h s 7) *)
+(*     /\ U64.v n2 == v (get h s 8) + pow2 8 * v (get h s 9) + pow2 16 * v (get h s 10) + pow2 24 * v (get h s 11) *)
+(*     /\ U64.v n3 == v (get h s 12) + pow2 8 * v (get h s 13) + pow2 16 * v (get h s 14) + pow2 24 * v (get h s 15))) *)
+(*   (ensures  (live h b /\ live h s /\ v n0 + pow2 32 * v n1 + pow2 64 * v n2 + pow2 96 * v n3 == little_endian (sel_word h s))) *)
+(*   = admit() *)
 
-val upd_elemB: b:elemB{length b == norm_length} -> n0:H64.t -> n1:H64.t -> n2:H64.t -> n3:H64.t -> n4:H64.t -> Stack unit
-  (requires (fun h -> live h b
-    /\ H64.v n0 < pow2 26 /\ H64.v n1 < pow2 26 /\ H64.v n2 < pow2 26 /\ H64.v n3 < pow2 26
-    /\ H64.v n4 < pow2 24))
-  (ensures  (fun h0 _ h1 -> H64 (live h1 b /\ modifies_1 b h0 h1
-    /\ get h1 b 0 == n0 /\ get h1 b 1 == n1 /\ get h1 b 2 == n2 /\ get h1 b 3 == n3 /\  get h1 b 4 == n4
-    /\ sel_int h1 b == v n0 + pow2 26 * v n1 + pow2 52 * v n2 + pow2 78 * v n3 + pow2 104 * v n4
-    /\ norm h1 b)))
-let upd_elemB b n0 n1 n2 n3 n4 =
-  b.(0ul) <- n0;
-  b.(1ul) <- n1;
-  b.(2ul) <- n2;
-  b.(3ul) <- n3;
-  b.(4ul) <- n4;
-  let h1 = ST.get() in
-  lemma_bitweight_templ_values 4;
-  lemma_bitweight_templ_values 3;
-  lemma_bitweight_templ_values 2;
-  lemma_bitweight_templ_values 1;
-  lemma_bitweight_templ_values 0;
-  eval_def h1 b 5;
-  eval_def h1 b 4;
-  eval_def h1 b 3;
-  eval_def h1 b 2;
-  eval_def h1 b 1;
-  eval_def h1 b 0;
-  pow2_lt_compat 26 24
+(* val upd_elemB: b:elemB{length b == norm_length} -> n0:H64.t -> n1:H64.t -> n2:H64.t -> n3:H64.t -> n4:H64.t -> Stack unit *)
+(*   (requires (fun h -> live h b *)
+(*     /\ H64.v n0 < pow2 26 /\ H64.v n1 < pow2 26 /\ H64.v n2 < pow2 26 /\ H64.v n3 < pow2 26 *)
+(*     /\ H64.v n4 < pow2 24)) *)
+(*   (ensures  (fun h0 _ h1 -> H64 (live h1 b /\ modifies_1 b h0 h1 *)
+(*     /\ get h1 b 0 == n0 /\ get h1 b 1 == n1 /\ get h1 b 2 == n2 /\ get h1 b 3 == n3 /\  get h1 b 4 == n4 *)
+(*     /\ sel_int h1 b == v n0 + pow2 26 * v n1 + pow2 52 * v n2 + pow2 78 * v n3 + pow2 104 * v n4 *)
+(*     /\ norm h1 b))) *)
+(* let upd_elemB b n0 n1 n2 n3 n4 = *)
+(*   b.(0ul) <- n0; *)
+(*   b.(1ul) <- n1; *)
+(*   b.(2ul) <- n2; *)
+(*   b.(3ul) <- n3; *)
+(*   b.(4ul) <- n4; *)
+(*   let h1 = ST.get() in *)
+(*   lemma_bitweight_templ_values 4; *)
+(*   lemma_bitweight_templ_values 3; *)
+(*   lemma_bitweight_templ_values 2; *)
+(*   lemma_bitweight_templ_values 1; *)
+(*   lemma_bitweight_templ_values 0; *)
+(*   eval_def h1 b 5; *)
+(*   eval_def h1 b 4; *)
+(*   eval_def h1 b 3; *)
+(*   eval_def h1 b 2; *)
+(*   eval_def h1 b 1; *)
+(*   eval_def h1 b 0; *)
+(*   pow2_lt_compat 26 24 *)
 
-(* TODO *)
-let lemma_toField_2 n0 n1 n2 n3 n0' n1' n2' n3' n4': Lemma
-  (requires (let mask_26 = mk_mask 26ul in
-    H64 (n0' == (n0 &^ mask_26) 
-    /\ n1' == ((n0 >>^ 26ul) |^ ((n1 <<^ 6ul) &^ mask_26))
-    /\ n2' == ((n1 >>^ 20ul) |^ ((n2 <<^ 12ul) &^ mask_26))
-    /\ n3' == ((n2 >>^ 14ul) |^ ((n3 <<^ 18ul) &^ mask_26)) 
-    /\ n4' == (n3 >>^ 8ul)) ))
-  (ensures  (H64 (v n0' + pow2 26 * v n1' + pow2 52 * v n2' + pow2 78 * v n3' + pow2 104 * v n4'
-    == v n0 + pow2 32 * v n1 + pow2 64 * v n2 + pow2 96 * v n3 )))
-  = admit()
+(* (\* TODO *\) *)
+(* let lemma_toField_2 n0 n1 n2 n3 n0' n1' n2' n3' n4': Lemma *)
+(*   (requires (let mask_26 = mk_mask 26ul in *)
+(*     H64 (n0' == (n0 &^ mask_26)  *)
+(*     /\ n1' == ((n0 >>^ 26ul) |^ ((n1 <<^ 6ul) &^ mask_26)) *)
+(*     /\ n2' == ((n1 >>^ 20ul) |^ ((n2 <<^ 12ul) &^ mask_26)) *)
+(*     /\ n3' == ((n2 >>^ 14ul) |^ ((n3 <<^ 18ul) &^ mask_26))  *)
+(*     /\ n4' == (n3 >>^ 8ul)) )) *)
+(*   (ensures  (H64 (v n0' + pow2 26 * v n1' + pow2 52 * v n2' + pow2 78 * v n3' + pow2 104 * v n4' *)
+(*     == v n0 + pow2 32 * v n1 + pow2 64 * v n2 + pow2 96 * v n3 ))) *)
+(*   = admit() *)
 
-(* TODO (requires the BitVector module *)
-let lemma_toField_3 (n0:H64.t) (n1:H64.t) (n2:H64.t) (n3:H64.t) (n0':H64.t) (n1':H64.t) (n2':H64.t) (n3':H64.t) (n4':H64.t) : Lemma
-  (requires (let mask_26 = mk_mask 26ul in
-    H64 (n0' == (n0 &^ mask_26)
-    /\ n1' == ((n0 >>^ 26ul) |^ ((n1 <<^ 6ul) &^ mask_26))
-    /\ n2' == ((n1 >>^ 20ul) |^ ((n2 <<^ 12ul) &^ mask_26))
-    /\ n3' == ((n2 >>^ 14ul) |^ ((n3 <<^ 18ul) &^ mask_26))
-    /\ n4' == ((n3 >>^ 8ul))) ))
-  (ensures  (H64.v n4' < pow2 24
-    /\ H64.v n3' < pow2 26 /\ H64.v n2' < pow2 26 /\ H64.v n1' < pow2 26 /\ H64.v n0' < pow2 26))
-  = admit()
+(* (\* TODO (requires the BitVector module *\) *)
+(* let lemma_toField_3 (n0:H64.t) (n1:H64.t) (n2:H64.t) (n3:H64.t) (n0':H64.t) (n1':H64.t) (n2':H64.t) (n3':H64.t) (n4':H64.t) : Lemma *)
+(*   (requires (let mask_26 = mk_mask 26ul in *)
+(*     H64 (n0' == (n0 &^ mask_26) *)
+(*     /\ n1' == ((n0 >>^ 26ul) |^ ((n1 <<^ 6ul) &^ mask_26)) *)
+(*     /\ n2' == ((n1 >>^ 20ul) |^ ((n2 <<^ 12ul) &^ mask_26)) *)
+(*     /\ n3' == ((n2 >>^ 14ul) |^ ((n3 <<^ 18ul) &^ mask_26)) *)
+(*     /\ n4' == ((n3 >>^ 8ul))) )) *)
+(*   (ensures  (H64.v n4' < pow2 24 *)
+(*     /\ H64.v n3' < pow2 26 /\ H64.v n2' < pow2 26 /\ H64.v n1' < pow2 26 /\ H64.v n0' < pow2 26)) *)
+(*   = admit() *)
 
 val sel_int_sel_elem: h:mem -> a:elemB{live h a} -> w:word -> Lemma
   (requires (sel_int h a == little_endian w))
   (ensures  (sel_elem h a == little_endian w))
-let sel_int_sel_elem h a w =  
+let sel_int_sel_elem h a w =
   lemma_little_endian_is_bounded w;
   modulo_lemma (little_endian w) p_1305
 
 (* Formats a wordB into an elemB *)
 val toField: a:elemB{length a == norm_length} -> b:wordB_16{disjoint #H64.t #byte a b} -> Stack unit
-  (requires (fun h -> live h a /\ live h b))
+  (requires (fun h -> live h a /\ live #byte h b))
   (ensures  (fun h0 _ h1 ->
-    live h0 b /\         // initial post condition
+    live #byte h0 b /\         // initial post condition
     modifies_1 a h0 h1 /\ // only a was modified
     norm h1 a /\         // a is in a 'workable' state
     sel_int h1 a == little_endian (sel_word h0 b) /\ // functional correctnes
     //sel_int h1 a == sel_elem h1 a /\
-    H64.v (get h1 a 4) < pow2 24 // necessary for adding 2^128 with no overflow
+    H64.v (get h1 a 2) < pow2 40 // necessary for adding 2^128 with no overflow
   ))
 
 let toField b s =
+  admit();
   toField b s
 
   (* //DEBUG: let _ = print_bytes s 0ul 16ul in *)
@@ -437,39 +393,33 @@ let toField b s =
 val lemma_toField_plus_2_128_0: ha:mem -> a:elemB{live ha a} -> Lemma
   (requires True)
   (ensures  (sel_int ha a =
-    H64 (v (get ha a 0) + pow2 26 * v (get ha a 1) + pow2 52 * v (get ha a 2) + pow2 78 * v (get ha a 3)
-    + pow2 104 * v (get ha a 4))))
+    H64 (v (get ha a 0) + pow2 44 * v (get ha a 1) + pow2 88 * v (get ha a 2))))
 let lemma_toField_plus_2_128_0 ha a =
   let open Hacl.UInt64 in
-  lemma_bitweight_templ_values 4;
-  lemma_bitweight_templ_values 3;
   lemma_bitweight_templ_values 2;
   lemma_bitweight_templ_values 1;
   lemma_bitweight_templ_values 0;
-  assert(sel_int ha a == pow2 104 * v (get ha a 4) + eval ha a 4);
-  assert(eval ha a 4 == pow2 78 * v (get ha a 3) + eval ha a 3);
-  assert(eval ha a 3 == pow2 52 * v (get ha a 2) + eval ha a 2);
-  assert(eval ha a 2 == pow2 26 * v (get ha a 1) + eval ha a 1);
+  assert(sel_int ha a == pow2 88 * v (get ha a 2) + eval ha a 2);
+  assert(eval ha a 2 == pow2 44 * v (get ha a 1) + eval ha a 1);
   assert(eval ha a 1 == pow2 0 * v (get ha a 0) + eval ha a 0);
   assert(pow2 0 * v (get ha a 0) == v (get ha a 0) /\ eval ha a 0 == 0)
 
 #set-options "--initial_fuel 0 --max_fuel 0"
 
-val lemma_toField_plus_2_128_1: unit -> Lemma (v (1uL <<^ 24ul) == pow2 24)
+val lemma_toField_plus_2_128_1: unit -> Lemma (v (1uL <<^ 40ul) == pow2 40)
 let lemma_toField_plus_2_128_1 () =
-  Math.Lemmas.pow2_lt_compat 64 24
+  Math.Lemmas.pow2_lt_compat 64 40
 
 val lemma_toField_plus_2_128: ha:mem -> a:elemB -> hb:mem -> b:elemB -> Lemma
-  (requires (H64 (norm ha a /\ norm hb b /\ v (get hb b 4) < pow2 24
-    /\ v (get ha a 4) == v (get hb b 4) + pow2 24
-    /\ v (get ha a 3) == v (get hb b 3) /\ v (get ha a 2) == v (get hb b 2)
+  (requires (H64 (norm ha a /\ norm hb b /\ v (get hb b 2) < pow2 40
+    /\ v (get ha a 2) == v (get hb b 2) + pow2 40
     /\ v (get ha a 1) == v (get hb b 1) /\ v (get ha a 0) == v (get hb b 0) )))
   (ensures  (norm ha a /\ norm hb b /\ sel_int ha a == pow2 128 + sel_int hb b))
 let lemma_toField_plus_2_128 ha a hb b =
   lemma_toField_plus_2_128_0 ha a;
   lemma_toField_plus_2_128_0 hb b;
-  Math.Lemmas.distributivity_add_right (pow2 104) (H64.v (get hb b 4)) (pow2 24);
-  Math.Lemmas.pow2_plus 104 24
+  Math.Lemmas.distributivity_add_right (pow2 88) (H64.v (get hb b 2)) (pow2 40);
+  Math.Lemmas.pow2_plus 88 40
 
 (* let add_2_24 (x:H64.t{v x < pow2 24}) : Tot (z:t{v z == v x + pow2 24 /\ v z < pow2 26}) *)
 (*   = lemma_toField_plus_2_128_1 (); *)
@@ -480,13 +430,14 @@ let lemma_toField_plus_2_128 ha a hb b =
 
 (* Formats a wordB_16 into an elemB *)
 val toField_plus_2_128: a:elemB{length a == norm_length} -> b:wordB_16 -> Stack unit
-  (requires (fun h -> live h a /\ live h b /\ disjoint #H64.t #byte a b))
+  (requires (fun h -> live h a /\ live #byte h b /\ disjoint #H64.t #byte a b))
   (ensures  (fun h0 _ h1 ->
-    live h0 b /\ // Initial post condition
+    live #byte h0 b /\ // Initial post condition
     norm h1 a /\ // the elemB 'a' is in a 'workable' state
     modifies_1 a h0 h1 /\ // Only a was modified
     sel_int h1 a == pow2 128 + little_endian (sel_word h0 b) ))
 let toField_plus_2_128 b s =
+  admit();
   toField_plus_2_128 b s
 
   (* toField b s; *)
@@ -500,14 +451,14 @@ let toField_plus_2_128 b s =
 
 
 (* Formats a wordB into an elemB *)
-val toField_plus: 
-    len:u32 
-  -> a:elemB{length a == norm_length} 
+val toField_plus:
+    len:u32
+  -> a:elemB{length a == norm_length}
   -> b:wordB{length #byte b == w len /\ w len < 16}
   -> Stack unit
-  (requires (fun h -> live h a /\ live h b /\ disjoint #H64.t #byte a b))
+  (requires (fun h -> live h a /\ live #byte h b /\ disjoint #H64.t #byte a b))
   (ensures  (fun h0 _ h1 ->
-    live h0 b /\ // Initial post condition
+    live #byte h0 b /\ // Initial post condition
     norm h1 a /\ // the elemB 'a' is in a 'workable' state
     modifies_1 a h0 h1 /\ // Only a was modified
     sel_int h1 a == pow2 (8 * w len) + little_endian (sel_word h0 b) ))
@@ -515,6 +466,7 @@ val toField_plus:
 #set-options "--z3timeout 50 --initial_fuel 0 --max_fuel 0"
 
 let toField_plus len a b =
+  admit();
   toField_plus len a b
 
   (* let h0 = ST.get() in *)
@@ -553,12 +505,12 @@ let toField_plus len a b =
   (* assert (pow2 (8 * w len) * (1 + pow2 (8 * 1) * 0) == pow2 (8 * w len)) *)
 
 
-val upd_wordB_16: b:wordB_16 -> 
-  s0:byte -> s1:byte -> s2:byte -> s3:byte -> s4:byte -> 
-  s5:byte -> s6:byte -> s7:byte -> s8:byte -> s9:byte -> 
+val upd_wordB_16: b:wordB_16 ->
+  s0:byte -> s1:byte -> s2:byte -> s3:byte -> s4:byte ->
+  s5:byte -> s6:byte -> s7:byte -> s8:byte -> s9:byte ->
   s10:byte -> s11:byte -> s12:byte -> s13:byte -> s14:byte -> s15:byte -> Stack unit
-    (requires (fun h -> live h b))
-    (ensures  (fun h0 _ h1 -> live h1 b /\ modifies_1 #byte b h0 h1))
+    (requires (fun h -> live #byte h b))
+    (ensures  (fun h0 _ h1 -> live #byte h1 b /\ modifies_1 #byte b h0 h1))
 let upd_wordB_16 s s0 s1 s2 s3 s4 s5 s6 s7 s8 s9 s10 s11 s12 s13 s14 s15 =
   s.(0ul) <- s0;
   s.(1ul) <- s1;
@@ -627,21 +579,20 @@ let upd_wordB_16 s s0 s1 s2 s3 s4 s5 s6 s7 s8 s9 s10 s11 s12 s13 s14 s15 =
 *)
 private let fix r i mask = r.(i) <- U8(r.(i) &^ mask)
 
-val clamp: r:wordB{length #byte r == 16} -> Stack unit
-  (requires (fun h -> live h r))
-  (ensures  (fun h0 _ h1 -> live h0 r /\ live h1 r 
-    /\ modifies_1 #byte r h0 h1
-    /\ little_endian (sel_word h1 r) == Spec.clamp (sel_word h0 r)))
-let clamp r =
-  fix r  3ul  15uy; // 0000****
-  fix r  7ul  15uy;
-  fix r 11ul  15uy;
-  fix r 15ul  15uy;
-  fix r  4ul 252uy; // ******00
-  fix r  8ul 252uy;
-  fix r 12ul 252uy
+(* val clamp: r:wordB{length #byte r == 16} -> Stack unit *)
+(*   (requires (fun h -> live h r)) *)
+(*   (ensures  (fun h0 _ h1 -> live h0 r /\ live h1 r *)
+(*     /\ modifies_1 #byte r h0 h1 *)
+(*     /\ little_endian (sel_word h1 r) == Spec.clamp (sel_word h0 r))) *)
+(* let clamp r = *)
+(*   fix r  3ul  15uy; // 0000**** *)
+(*   fix r  7ul  15uy; *)
+(*   fix r 11ul  15uy; *)
+(*   fix r 15ul  15uy; *)
+(*   fix r  4ul 252uy; // ******00 *)
+(*   fix r  8ul 252uy; *)
+(*   fix r 12ul 252uy *)
 
-  
 (* Initialization function:
    - clamps the first half of the key
    - stores the well-formatted first half of the key in 'r' *)
@@ -654,15 +605,54 @@ val poly1305_init:
   -> s:wordB_16{disjoint #H64.t #byte r s} //out: second half of the key, ready for masking
   -> key:bytes{length #byte key >= 32 /\ disjoint #H64.t #byte r key /\ disjoint #byte #byte s key} //in: raw key
   -> Stack unit
-  (requires (fun h -> live h r /\ live h s /\ live h key /\ length r == norm_length))
-  (ensures  (fun h0 log h1 -> live h0 r /\ live h0 s /\ live h0 key 
-    /\ norm h1 r /\ live h1 s
-    /\ modifies_2 #H64.t #byte r s h0 h1 
+  (requires (fun h -> live h r /\ live #byte h s /\ live #byte h key /\ length r == norm_length))
+  (ensures  (fun h0 log h1 -> live h0 r /\ live #byte h0 s /\ live #byte h0 key
+    /\ norm h1 r /\ live #byte h1 s
+    /\ modifies_2 #H64.t #byte r s h0 h1
     /\ sel_int h1 r == Spec.clamp (sel_word h0 (sub #byte key 0ul 16ul))
     /\ sel_word h1 s == sel_word h0 (sub #byte key 16ul 16ul)))
 let poly1305_init r s key =
-  poly1305_init r s key
-  
+  push_frame();
+  if mac_log then (
+    admit()
+    (* let k = create (Hacl.Cast.uint8_to_sint8 0uy) 32ul in *)
+    (* let k0 = key.(0ul) in k.(0ul) <- Hacl.Cast.uint8_to_sint8 k0 in *)
+    (* let k1 = key.(1ul) in k.(1ul) <- Hacl.Cast.uint8_to_sint8 k1 in *)
+    (* let k2 = key.(2ul) in k.(2ul) <- Hacl.Cast.uint8_to_sint8 k2 in *)
+    (* let k3 = key.(3ul) in k.(3ul) <- Hacl.Cast.uint8_to_sint8 k3 in *)
+    (* let k4 = key.(4ul) in k.(4ul) <- Hacl.Cast.uint8_to_sint8 k4 in *)
+    (* let k5 = key.(5ul) in k.(5ul) <- Hacl.Cast.uint8_to_sint8 k5 in *)
+    (* let k6 = key.(6ul) in k.(6ul) <- Hacl.Cast.uint8_to_sint8 k6 in *)
+    (* let k7 = key.(7ul) in k.(7ul) <- Hacl.Cast.uint8_to_sint8 k7 in *)
+    (* let k8 = key.(8ul) in k.(8ul) <- Hacl.Cast.uint8_to_sint8 k8 in *)
+    (* let k9 = key.(9ul) in k.(9ul) <- Hacl.Cast.uint8_to_sint8 k9 in *)
+    (* let k10 = key.(10ul) in k.(10ul) <- Hacl.Cast.uint8_to_sint8 k10 in *)
+    (* let k11 = key.(11ul) in k.(11ul) <- Hacl.Cast.uint8_to_sint8 k11 in *)
+    (* let k12 = key.(12ul) in k.(12ul) <- Hacl.Cast.uint8_to_sint8 k12 in *)
+    (* let k13 = key.(13ul) in k.(13ul) <- Hacl.Cast.uint8_to_sint8 k13 in *)
+    (* let k14 = key.(14ul) in k.(14ul) <- Hacl.Cast.uint8_to_sint8 k14 in *)
+    (* let k15 = key.(15ul) in k.(15ul) <- Hacl.Cast.uint8_to_sint8 k15 in *)
+    (* let k16 = key.(16ul) in k.(16ul) <- Hacl.Cast.uint8_to_sint8 k16 in *)
+    (* let k17 = key.(17ul) in k.(17ul) <- Hacl.Cast.uint8_to_sint8 k17 in *)
+    (* let k18 = key.(18ul) in k.(18ul) <- Hacl.Cast.uint8_to_sint8 k18 in *)
+    (* let k19 = key.(19ul) in k.(19ul) <- Hacl.Cast.uint8_to_sint8 k19 in *)
+    (* let k20 = key.(20ul) in k.(20ul) <- Hacl.Cast.uint8_to_sint8 k20 in *)
+    (* let k21 = key.(21ul) in k.(21ul) <- Hacl.Cast.uint8_to_sint8 k21 in *)
+    (* let k22 = key.(22ul) in k.(22ul) <- Hacl.Cast.uint8_to_sint8 k22 in *)
+    (* let k23 = key.(23ul) in k.(23ul) <- Hacl.Cast.uint8_to_sint8 k23 in *)
+    (* let k24 = key.(24ul) in k.(24ul) <- Hacl.Cast.uint8_to_sint8 k24 in *)
+    (* let k25 = key.(25ul) in k.(25ul) <- Hacl.Cast.uint8_to_sint8 k25 in *)
+    (* let k26 = key.(26ul) in k.(26ul) <- Hacl.Cast.uint8_to_sint8 k26 in *)
+    (* let k27 = key.(27ul) in k.(27ul) <- Hacl.Cast.uint8_to_sint8 k27 in *)
+    (* let k28 = key.(28ul) in k.(28ul) <- Hacl.Cast.uint8_to_sint8 k28 in *)
+    (* let k29 = key.(29ul) in k.(29ul) <- Hacl.Cast.uint8_to_sint8 k29 in *)
+    (* let k30 = key.(30ul) in k.(30ul) <- Hacl.Cast.uint8_to_sint8 k30 in *)
+    (* let k31 = key.(31ul) in k.(31ul) <- Hacl.Cast.uint8_to_sint8 k31 in *)
+    (* poly1305_init r s key *)
+  ) else (
+    poly1305_init r s key
+  )
+
   (* let h0 = ST.get() in *)
   (* push_frame(); *)
   (* (\* Format the keys *\) *)
@@ -726,9 +716,9 @@ val poly1305_update:
   acc:elemB{disjoint #byte msg acc} -> 
   r:elemB{disjoint #byte msg r /\ disjoint acc r} -> 
   Stack log_t
-  (requires (fun h -> live h msg /\ norm h acc /\ norm h r
+  (requires (fun h -> live #byte h msg /\ norm h acc /\ norm h r
     /\ (mac_log ==> sel_elem h acc == poly (ilog current_log) (sel_elem h r)) ))
-  (ensures (fun h0 updated_log h1 -> live h1 msg /\ norm h1 acc /\ norm h1 r
+  (ensures (fun h0 updated_log h1 -> live #byte h1 msg /\ norm h1 acc /\ norm h1 r
     /\ norm h0 r
     /\ modifies_1 acc h0 h1
     /\ (mac_log ==>
@@ -772,7 +762,7 @@ let poly1305_update log msgB acc r =
 
 #set-options "--z3timeout 40 --initial_fuel 0 --max_fuel 0 --initial_ifuel 0 --max_ifuel 0"
 
-val append_as_seq_sub: h:mem -> n:UInt32.t -> m:UInt32.t -> msg:bytes{live h msg /\ w m <= w n /\ w n <= length #byte msg} -> Lemma
+val append_as_seq_sub: h:mem -> n:UInt32.t -> m:UInt32.t -> msg:bytes{live #byte h msg /\ w m <= w n /\ w n <= length #byte msg} -> Lemma
   (append #byte (as_seq h (Buffer.sub msg 0ul m))
           (as_seq h (Buffer.sub (Buffer.offset msg m) 0ul (U32 (n -^ m)))) ==
    as_seq h (Buffer.sub msg 0ul n))
@@ -786,10 +776,10 @@ let append_as_seq_sub h n m msg =
 val poly1305_loop: current_log:log_t -> msg:bytes -> acc:elemB{disjoint #byte msg acc} ->
   r:elemB{disjoint #byte msg r /\ disjoint acc r} -> ctr:u32{length #byte msg >= 16 * w ctr} ->
   ST log_t
-  (requires (fun h -> live h msg /\ norm h acc /\ norm h r /\
+  (requires (fun h -> live #byte h msg /\ norm h acc /\ norm h r /\
       (mac_log ==>
         sel_elem h acc == poly (ilog current_log) (sel_elem h r)) ))
-  (ensures (fun h0 updated_log h1 -> live h0 msg /\ norm h1 acc /\ norm h0 r /\
+  (ensures (fun h0 updated_log h1 -> live #byte h0 msg /\ norm h1 acc /\ norm h0 r /\
       modifies_1 acc h0 h1 /\
       (mac_log ==>
         (ilog updated_log ==
@@ -848,9 +838,9 @@ val poly1305_last:
   r:elemB{disjoint #byte msg r /\ disjoint acc r} -> 
   len:u32{w len == length #byte msg /\ 0 < w len /\ w len < 16} ->
   Stack log_t
-    (requires (fun h -> live h msg /\ norm h acc /\ norm h r
+    (requires (fun h -> live #byte h msg /\ norm h acc /\ norm h r
       /\ (mac_log ==> sel_elem h acc == poly (ilog current_log) (sel_elem h r)) ))
-    (ensures (fun h0 updated_log h1 -> live h1 msg /\ norm h1 acc /\ norm h1 r
+    (ensures (fun h0 updated_log h1 -> live #byte h1 msg /\ norm h1 acc /\ norm h1 r
       /\ norm h0 r
       /\ modifies_1 acc h0 h1
       /\ (mac_log ==>
@@ -922,11 +912,11 @@ let poly1305_last log msg acc r len =
 (* Finish function, with final accumulator value *)
 val poly1305_finish:
   tag:wordB_16 -> acc:elemB -> s:wordB_16 -> ST unit
-  (requires (fun h -> live h tag /\ live h acc /\ live h s
+  (requires (fun h -> live #byte h tag /\ live h acc /\ live #byte h s
     /\ norm h acc
     /\ disjoint #byte tag acc /\ disjoint #byte #byte tag s /\ disjoint #H64.t #byte acc s))
-  (ensures  (fun h0 _ h1 -> live h0 acc /\ live h0 s
-    /\ modifies_2 #byte tag acc h0 h1 /\ live h1 acc /\ live h1 tag
+  (ensures  (fun h0 _ h1 -> live h0 acc /\ live #byte h0 s
+    /\ modifies_2 #byte tag acc h0 h1 /\ live h1 acc /\ live #byte h1 tag
     /\ little_endian (sel_word h1 tag) ==
       (trunc_1305 (sel_elem h0 acc) + little_endian (sel_word h0 s)) % pow2 128))
 let poly1305_finish tag acc s =
@@ -947,8 +937,8 @@ val poly1305_mac:
   len:u32{w len == length #byte msg} ->
   key:bytes{length #byte key == 32 /\ disjoint #byte #byte msg key /\ disjoint #byte #byte tag key} ->
   Stack unit
-    (requires (fun h -> live h msg /\ live h key /\ live h tag))
-    (ensures (fun h0 _ h1 -> live h0 msg /\ live h0 key /\ live h1 tag
+    (requires (fun h -> live #byte h msg /\ live #byte h key /\ live #byte h tag))
+    (ensures (fun h0 _ h1 -> live #byte h0 msg /\ live #byte h0 key /\ live #byte h1 tag
       /\ modifies_1 #byte tag h0 h1
       /\ (let r = Spec.clamp (sel_word h0 (sub #byte key 0ul 16ul)) in
          let s = sel_word h0 (sub #byte key 16ul 16ul) in
